test/TestPipeline.v
@@ -1,0 +1,5 @@
+From MetaRocq.Template Require Import All.
+From Hallmark Require Import Pipeline.
+From HallmarkExamples Require Import Allowed.
+
+MetaRocq Run (hallmark_pipeline allowed).
