theories/Lookup.v
@@ -5,10 +5,28 @@
     inductive declaration. *)
 
 From MetaRocq.Template Require Import All.
+From Stdlib Require Import List.
+Import ListNotations.
 
 Definition find_inductive (Σ : global_env) (kn : kername)
   : option mutual_inductive_body :=
   match lookup_env Σ kn with
   | Some (InductiveDecl mib) => Some mib
+  | _ => None
+  end.
+
+(** Look up a constructor's name from the global environment. *)
+Definition lookup_constructor_name (Σ : global_env) (ind : inductive) (cidx : nat)
+  : option ident :=
+  match lookup_env Σ (inductive_mind ind) with
+  | Some (InductiveDecl mib) =>
+    match nth_error (ind_bodies mib) (inductive_ind ind) with
+    | Some oib =>
+      match nth_error (ind_ctors oib) cidx with
+      | Some cdecl => Some (cstr_name cdecl)
+      | None => None
+      end
+    | None => None
+    end
   | _ => None
   end.
